executable.v
@@ -10,21 +10,21 @@ Definition assign_exec (Γ : env Ti) (m : mem Ti) (a : addr Ti)
     (v : val Ti) (ass : assign) : option (val Ti * val Ti) :=
   match ass with
   | Assign =>
-     guard (val_cast_ok Γ (memenv_of m) (type_of a) v);
+     guard (val_cast_ok Γ ('{m}) (type_of a) v);
      let v' := val_cast (type_of a) v in
      Some (v',v')
   | PreOp op =>
      va ← m !!{Γ} a;
-     guard (val_binop_ok Γ (memenv_of m) op va v);
+     guard (val_binop_ok Γ ('{m}) op va v);
      let v' := val_binop Γ op va v in
-     guard (val_cast_ok Γ (memenv_of m) (type_of a) v');
+     guard (val_cast_ok Γ ('{m}) (type_of a) v');
      let v'' := val_cast (type_of a) v' in
      Some (v'', v'')
   | PostOp op =>
      va ← m !!{Γ} a;
-     guard (val_binop_ok Γ (memenv_of m) op va v);
+     guard (val_binop_ok Γ ('{m}) op va v);
      let v' := val_binop Γ op va v in
-     guard (val_cast_ok Γ (memenv_of m) (type_of a) v');
+     guard (val_cast_ok Γ ('{m}) (type_of a) v');
      Some (va, val_cast (type_of a) v')
   end.
 Definition ehstep_exec (Γ : env Ti) (ρ : stack)
@@ -55,13 +55,13 @@ Definition ehstep_exec (Γ : env Ti) (ρ : stack)
      guard (mem_freeable a m);
      Some (#{Ω} voidV, mem_free (addr_index a) m)
   | @{op} #{Ω} v =>
-     guard (val_unop_ok (memenv_of m) op v);
+     guard (val_unop_ok ('{m}) op v);
      Some (#{Ω} (val_unop op v), m)
   | #{Ωl} vl @{op} #{Ωr} vr =>
-     guard (val_binop_ok Γ (memenv_of m) op vl vr);
+     guard (val_binop_ok Γ ('{m}) op vl vr);
      Some (#{Ωl ∪ Ωr} (val_binop Γ op vl vr), m)
   | if{#{Ω} v} e2 else e3 =>
-     match val_true_false_dec (memenv_of m) v with
+     match val_true_false_dec ('{m}) v with
      | inleft (left _) => Some (e2, mem_unlock Ω m)
      | inleft (right _) => Some (e3, mem_unlock Ω m)
      | inright _ => None
@@ -69,7 +69,7 @@ Definition ehstep_exec (Γ : env Ti) (ρ : stack)
   | #{Ω} v,, er =>
      Some (er, mem_unlock Ω m)
   | cast{τ} (#{Ω} v) =>
-     guard (val_cast_ok Γ (memenv_of m) τ v);
+     guard (val_cast_ok Γ ('{m}) τ v);
      Some (#{Ω} (val_cast τ v), m)
   | _ => None
   end%E.
@@ -162,7 +162,7 @@ Definition cstep_exec (Γ : env Ti) (δ : funenv Ti)
       | CExpr e (ret □) :: k =>
          {[ State k (Stmt (⇈ v) (ret e)) (mem_unlock Ω m) ]}
       | CExpr e (while{□} s) :: k =>
-        match val_true_false_dec (memenv_of m) v with
+        match val_true_false_dec ('{m}) v with
         | inleft (left _) =>
            {[ State (CStmt (while{e} □) :: k) (Stmt ↘ s) (mem_unlock Ω m) ]}
         | inleft (right _) =>
@@ -170,7 +170,7 @@ Definition cstep_exec (Γ : env Ti) (δ : funenv Ti)
         | inright _ => {[ State k (Undef (UndefBranch e (while{□} s) Ω v)) m ]}
          end
       | CExpr e (if{□} s1 else s2) :: k =>
-        match val_true_false_dec (memenv_of m) v with
+        match val_true_false_dec ('{m}) v with
         | inleft (left _) =>
            {[State (CStmt (if{e} □ else s2) :: k) (Stmt ↘ s1) (mem_unlock Ω m)]}
         | inleft (right _) =>
