frontend.v
@@ -138,7 +138,7 @@ Fixpoint lookup_var (m : mem Ti) (x : N)
   | [] => None
   | (y,Global o) :: xs =>
      if decide (x = y)
-     then τ ← type_check (memenv_of m) o; Some (% (addr_top o τ), inl τ)
+     then τ ← type_check ('{m}) o; Some (% (addr_top o τ), inl τ)
      else lookup_var m x i xs
   | (y,Local τ) :: xs =>
      if decide (x = y) then Some (var{τ} i, inl τ)
@@ -691,7 +691,7 @@ Proof. induction 1 as [|[? []]]; simpl; auto. Qed.
 
 Lemma to_R_typed Γ Γf m τs e τlr e' τ' :
   ✓ Γ → ✓{Γ} Γf → ✓{Γ}* τs → to_R (e,τlr) = (e',τ') →
-  (Γ,Γf,memenv_of m,τs) ⊢ e : τlr → (Γ,Γf,memenv_of m,τs) ⊢ e' : inr τ'.
+  (Γ,Γf,'{m},τs) ⊢ e : τlr → (Γ,Γf,'{m},τs) ⊢ e' : inr τ'.
 Proof.
   unfold to_R; intros; destruct τlr as [τl|τr]; simplify_equality'; auto.
   destruct (maybe_TArray τl) as [[τ n]|] eqn:Hτ; simplify_equality'.
@@ -703,7 +703,7 @@ Qed.
 Lemma to_R_NULL_typed Γ Γf m τs σ e τlr e' τ' :
   ✓ Γ → ✓{Γ} Γf → ✓{Γ}* τs →
   to_R_NULL σ (e,τlr) = (e',τ') → ptr_type_valid Γ σ →
-  (Γ,Γf,memenv_of m,τs) ⊢ e : τlr → (Γ,Γf,memenv_of m,τs) ⊢ e' : inr τ'.
+  (Γ,Γf,'{m},τs) ⊢ e : τlr → (Γ,Γf,'{m},τs) ⊢ e' : inr τ'.
 Proof.
   unfold to_R_NULL. destruct (to_R (e,τlr)) as [e'' τ''] eqn:?.
   destruct 5 as [σb Hσb| |]; simplify_equality'; eauto 2 using to_R_typed.
@@ -713,10 +713,10 @@ Qed.
 
 Lemma var_lookup_typed Γ Γf m xs x e τlr :
   ✓ Γ → ✓{Γ} m → var_env_valid Γ xs → lookup_var m x 0 xs = Some (e,τlr) →
-  (Γ,Γf,memenv_of m,var_env_stack_types xs) ⊢ e : τlr.
+  (Γ,Γf,'{m},var_env_stack_types xs) ⊢ e : τlr.
 Proof.
   intros ?? Hxs. cut (∀ τs', lookup_var m x (length τs') xs = Some (e,τlr) →
-    (Γ,Γf,memenv_of m,τs' ++ var_env_stack_types xs) ⊢ e : τlr).
+    (Γ,Γf,'{m},τs' ++ var_env_stack_types xs) ⊢ e : τlr).
   { intros help. apply (help []). }
   induction Hxs as [|[x' [o|τ|τi z|]] ? xs ? IH];
     intros τs' ?; simplify_option_equality; simplify_type_equality; eauto 2.
@@ -730,8 +730,8 @@ Qed.
 Lemma convert_ptrs_typed Γ Γf m τs e1 τ1 e2 τ2 e1' e2' τ' :
   ✓ Γ → ✓{Γ} Γf → ✓{Γ}* τs →
   convert_ptrs (e1,τ1) (e2,τ2) = Some (e1', e2', τ') →
-  (Γ,Γf,memenv_of m,τs) ⊢ e1 : inr τ1 → (Γ,Γf,memenv_of m,τs) ⊢ e2 : inr τ2 →
-  (Γ,Γf,memenv_of m,τs) ⊢ e1' : inr τ' ∧ (Γ,Γf,memenv_of m,τs) ⊢ e2' : inr τ'.
+  (Γ,Γf,'{m},τs) ⊢ e1 : inr τ1 → (Γ,Γf,'{m},τs) ⊢ e2 : inr τ2 →
+  (Γ,Γf,'{m},τs) ⊢ e1' : inr τ' ∧ (Γ,Γf,'{m},τs) ⊢ e2' : inr τ'.
 Proof.
   unfold convert_ptrs; destruct τ1 as [[|τp1|]| |], τ2 as [[|τp2|]| |]; intros;
     simplify_option_equality; split; repeat typed_constructor;
@@ -740,9 +740,8 @@ Qed.
 Lemma to_if_expr_typed Γ Γf m τs e1 τb e2 τ2 e3 τ3 e τlr :
   ✓ Γ → ✓{Γ} Γf → ✓{Γ}* τs →
   to_if_expr e1 (e2,τ2) (e3,τ3) = Some (e,τlr) →
-  (Γ,Γf,memenv_of m,τs) ⊢ e1 : inr (baseT τb) →
-  (Γ,Γf,memenv_of m,τs) ⊢ e2 : inr τ2 →
-  (Γ,Γf,memenv_of m,τs) ⊢ e3 : inr τ3 → (Γ,Γf,memenv_of m,τs) ⊢ e : τlr.
+  (Γ,Γf,'{m},τs) ⊢ e1 : inr (baseT τb) → (Γ,Γf,'{m},τs) ⊢ e2 : inr τ2 →
+  (Γ,Γf,'{m},τs) ⊢ e3 : inr τ3 → (Γ,Γf,'{m},τs) ⊢ e : τlr.
 Proof.
   unfold to_if_expr; intros;
     repeat match goal with
@@ -756,8 +755,8 @@ Qed.
 Lemma to_binop_expr_typed Γ Γf m τs op e1 τ1 e2 τ2 e τlr :
   ✓ Γ → ✓{Γ} Γf → ✓{Γ}* τs →
   to_binop_expr op (e1,τ1) (e2,τ2) = Some (e,τlr) →
-  (Γ,Γf,memenv_of m,τs) ⊢ e1 : inr τ1 → (Γ,Γf,memenv_of m,τs) ⊢ e2 : inr τ2 →
-  (Γ,Γf,memenv_of m,τs) ⊢ e : τlr.
+  (Γ,Γf,'{m},τs) ⊢ e1 : inr τ1 → (Γ,Γf,'{m},τs) ⊢ e2 : inr τ2 →
+  (Γ,Γf,'{m},τs) ⊢ e : τlr.
 Proof.
   unfold to_binop_expr; intros;
     repeat match goal with
@@ -771,7 +770,7 @@ Qed.
 Lemma to_expr_type_typed Γn Γ Γf m xs :
   ✓ Γ → ✓{Γ} Γf → ✓{Γ} m → var_env_valid Γ xs →
   (∀ ce e τlr, to_expr Γn Γ Γf m xs ce = inr (e,τlr) →
-    (Γ,Γf,memenv_of m,var_env_stack_types xs) ⊢ e : τlr) ∧
+    (Γ,Γf,'{m},var_env_stack_types xs) ⊢ e : τlr) ∧
   (∀ cτ,
     (∀ τ, to_type Γn Γ Γf m xs false cτ = inr τ → ✓{Γ} τ) ∧
     (∀ τ, to_type Γn Γ Γf m xs true cτ = inr τ → ptr_type_valid Γ τ)).
@@ -779,10 +778,10 @@ Proof.
   intros ????. assert (∀ f ces τs τ eτlrs,
      Γf !! f = Some (τs, τ) →
      Forall (λ ce, ∀ e τlr, to_expr Γn Γ Γf m xs ce = inr (e,τlr) →
-       (Γ,Γf,memenv_of m,var_env_stack_types xs) ⊢ e : τlr) ces →
+       (Γ,Γf,'{m},var_env_stack_types xs) ⊢ e : τlr) ces →
      Forall2 (cast_typed Γ) (snd <$> zip_with to_R_NULL τs eτlrs) τs →
      mapM (to_expr Γn Γ Γf m xs) ces = inr eτlrs →
-     (Γ,Γf,memenv_of m,var_env_stack_types xs) ⊢*
+     (Γ,Γf,'{m},var_env_stack_types xs) ⊢*
        cast{τs}* (fst <$> zip_with to_R_NULL τs eτlrs) :* inr <$> τs).
   { intros f ces τs τ eτlrs. rewrite mapM_inr. intros Hf ? Hcast Hces.
     assert (Forall (ptr_type_valid Γ) τs) as Hτs by eauto using Forall_impl,
@@ -836,7 +835,7 @@ Qed.
 Lemma to_expr_typed Γn Γ Γf m xs ce e τlr :
   ✓ Γ → ✓{Γ} Γf → ✓{Γ} m → var_env_valid Γ xs →
   to_expr Γn Γ Γf m xs ce = inr (e,τlr) →
-  (Γ,Γf,memenv_of m,var_env_stack_types xs) ⊢ e : τlr.
+  (Γ,Γf,'{m},var_env_stack_types xs) ⊢ e : τlr.
 Proof. intros. eapply to_expr_type_typed; eauto. Qed.
 Lemma to_type_valid Γn Γ Γf m xs cτ τ :
   ✓ Γ → ✓{Γ} Γf → ✓{Γ} m → var_env_valid Γ xs →
@@ -851,7 +850,7 @@ Lemma alloc_global_typed Γn Γ m xs x τ mce m' xs' :
   ✓ Γ → alloc_global Γn Γ m xs x τ mce = inr (m',xs') →
   ✓{Γ} m → var_env_valid Γ xs → ✓{Γ} τ →
   (**i 1.) *) ✓{Γ} m' ∧
-  (**i 2.) *) (∀ o σ, memenv_of m ⊢ o : σ → memenv_of m' ⊢ o : σ) ∧
+  (**i 2.) *) (∀ o σ, '{m} ⊢ o : σ → '{m'} ⊢ o : σ) ∧
   (**i 3.) *) var_env_valid Γ xs' ∧
   (**i 4.) *) var_env_stack_types xs = var_env_stack_types xs'.
 Proof.
@@ -864,7 +863,7 @@ Proof.
     repeat case_error_guard; simplify_equality'.
     destruct (⟦ e' ⟧ Γ ∅ [] m) as [[?|v]|] eqn:?; simplify_equality'.
     repeat case_option_guard; simplify_equality'.
-    assert ((Γ,memenv_of m) ⊢ inr v : inr τ'); [|typed_inversion_all].
+    assert ((Γ,'{m}) ⊢ inr v : inr τ'); [|typed_inversion_all].
     { eapply (expr_eval_typed_aux Γ ∅ [] (var_env_stack_types xs) ∅);
         eauto using to_R_NULL_typed, type_valid_ptr_type_valid, to_expr_typed,
         prefix_of_nil, funtypes_valid_empty, var_env_stack_types_valid.
@@ -878,9 +877,9 @@ Qed.
 Lemma to_stmt_typed Γn Γ Γf τret m xs Ls mLc mLb cs m' s cmτ :
   ✓ Γ → ✓{Γ} Γf → ✓{Γ} m → var_env_valid Γ xs →
   to_stmt Γn Γ Γf τret m xs Ls mLc mLb cs = inr (m',s,cmτ) →
-  (**i 1.) *) (Γ,Γf,memenv_of m',var_env_stack_types xs) ⊢ s : cmτ ∧
+  (**i 1.) *) (Γ,Γf,'{m'},var_env_stack_types xs) ⊢ s : cmτ ∧
   (**i 2.) *) ✓{Γ} m' ∧
-  (**i 3.) *) (∀ o σ, memenv_of m ⊢ o : σ → memenv_of m' ⊢ o : σ).
+  (**i 3.) *) (∀ o σ, '{m} ⊢ o : σ → '{m'} ⊢ o : σ).
 Proof.
   intros ??. revert m m' s cmτ xs Ls mLc mLb. induction cs; intros;
     repeat match goal with
@@ -934,7 +933,7 @@ Lemma to_envs_go_typed Θ Γn Γ Γf δ m xs :
   to_envs_go Θ = inr (Γn,Γ,Γf,δ,m,xs) →
   (**i 1.) *) ✓ Γ ∧
   (**i 2.) *) ✓{Γ} Γf ∧
-  (**i 3.) *) funenv_pretyped Γ (memenv_of m) δ Γf ∧
+  (**i 3.) *) funenv_pretyped Γ ('{m}) δ Γf ∧
   (**i 4.) *) ✓{Γ} m ∧
   (**i 5.) *) var_env_valid Γ xs ∧
   (**i 6.) *) var_env_stack_types xs = [].
@@ -997,7 +996,7 @@ Proof.
       funenv_pretyped_insert, to_types_valid, to_type_valid.
 Qed.
 Lemma to_envs_typed Θ Γ Γf δ m :
-  to_envs Θ = inr (Γ,Γf,δ,m) → ✓ Γ ∧ (Γ,memenv_of m) ⊢ δ : Γf ∧ ✓{Γ} m.
+  to_envs Θ = inr (Γ,Γf,δ,m) → ✓ Γ ∧ (Γ,'{m}) ⊢ δ : Γf ∧ ✓{Γ} m.
 Proof.
   unfold to_envs. intros. destruct (to_envs_go _)
     as [|[[[[[Γn Γ2] Γf2] δ2] m2] xs]] eqn:?; simplify_error_equality.
