type_preservation.v
@@ -20,31 +20,31 @@ Hint Extern 0 (_ ⊢ _ : _) => typed_constructor.
 Hint Extern 0 (_ ⊢ _ : _ ↣ _) => typed_constructor.
 
 Lemma initial_state_typed Γ Γf δ m f vs σs σ :
-  ✓{Γ} m → (Γ,memenv_of m) ⊢ δ : Γf → Γf !! f = Some (σs,σ) →
-  (Γ,memenv_of m) ⊢* vs :* σs → (Γ,Γf) ⊢ initial_state m f vs : f.
+  ✓{Γ} m → (Γ,'{m}) ⊢ δ : Γf → Γf !! f = Some (σs,σ) →
+  (Γ,'{m}) ⊢* vs :* σs → (Γ,Γf) ⊢ initial_state m f vs : f.
 Proof. eexists (Fun_type f); simpl; eauto. Qed.
 Lemma assign_preservation_1 Γ m ass a v v' va' τ1 τ2 σ :
   ✓ Γ → ✓{Γ} m → assign_typed Γ τ1 τ2 ass σ →
-  (Γ,memenv_of m) ⊢ a : τ1 → (Γ,memenv_of m) ⊢ v : τ2 →
-  assign_sem Γ m a v ass v' va' → (Γ,memenv_of m) ⊢ v' : σ.
+  (Γ,'{m}) ⊢ a : τ1 → (Γ,'{m}) ⊢ v : τ2 →
+  assign_sem Γ m a v ass v' va' → (Γ,'{m}) ⊢ v' : σ.
 Proof.
   destruct 3; inversion 3; simplify_type_equality';
     eauto using val_cast_typed, val_binop_typed, mem_lookup_typed.
 Qed.
 Lemma assign_preservation_2 Γ m ass a v v' va' τ1 τ2 σ :
   ✓ Γ → ✓{Γ} m → assign_typed Γ τ1 τ2 ass σ →
-  (Γ,memenv_of m) ⊢ a : τ1 → (Γ,memenv_of m) ⊢ v : τ2 →
-  assign_sem Γ m a v ass v' va' → (Γ,memenv_of m) ⊢ va' : τ1.
+  (Γ,'{m}) ⊢ a : τ1 → (Γ,'{m}) ⊢ v : τ2 →
+  assign_sem Γ m a v ass v' va' → (Γ,'{m}) ⊢ va' : τ1.
 Proof.
   destruct 3; inversion 3; simplify_type_equality';
     eauto using val_cast_typed, val_binop_typed, mem_lookup_typed.
 Qed.
 Lemma ehstep_preservation Γ Γf m1 m2 ρ τs e1 e2 τlr :
   ✓ Γ → Γ\ ρ ⊢ₕ e1, m1 ⇒ e2, m2 →
-  ✓{Γ} m1 → (Γ,Γf,memenv_of m1,τs) ⊢ e1 : τlr → memenv_of m1 ⊢* ρ :* τs →
+  ✓{Γ} m1 → (Γ,Γf,'{m1},τs) ⊢ e1 : τlr → '{m1} ⊢* ρ :* τs →
   (**i 1.) *) ✓{Γ} m2 ∧
-  (**i 2.) *) (Γ,Γf,memenv_of m2,τs) ⊢ e2 : τlr ∧
-  (**i 3.) *) ∀ o σ, memenv_of m1 ⊢ o : σ → memenv_of m2 ⊢ o : σ.
+  (**i 2.) *) (Γ,Γf,'{m2},τs) ⊢ e2 : τlr ∧
+  (**i 3.) *) ∀ o σ, '{m1} ⊢ o : σ → '{m2} ⊢ o : σ.
 Proof.
   intros ? [] ???.
   * typed_inversion_all; decompose_Forall_hyps; split_ands; auto.
@@ -95,20 +95,19 @@ Proof.
       eauto using val_cast_typed.
 Qed.
 Lemma cstep_preservation Γ Γf δ S1 S2 f :
-  ✓ Γ → Γ\ δ ⊢ₛ S1 ⇒ S2 →
-  (Γ,Γf) ⊢ S1 : f → (Γ,memenv_of (SMem S1)) ⊢ δ : Γf →
-  (Γ,Γf) ⊢ S2 : f ∧ (Γ,memenv_of (SMem S2)) ⊢ δ : Γf.
+  ✓ Γ → Γ\ δ ⊢ₛ S1 ⇒ S2 → (Γ,Γf) ⊢ S1 : f → (Γ,'{SMem S1}) ⊢ δ : Γf →
+  (Γ,Γf) ⊢ S2 : f ∧ (Γ,'{SMem S2}) ⊢ δ : Γf.
 Proof.
   intros ? p. case p; clear p.
   * intros m k (τf&HS&?&?) ?; typed_inversion_all; split; auto.
   * intros m k l (τf&HS&?&?) ?; typed_inversion_all; split; auto.
   * intros m k l (τf&HS&?&?) ?; typed_inversion_all; split; auto.
   * intros m k Ee e (τf&HS&?&?) ?; typed_inversion HS; split; auto.
-    edestruct (esctx_item_subst_typed_rev Γ Γf (memenv_of m)
+    edestruct (esctx_item_subst_typed_rev Γ Γf ('{m})
       (get_stack_types k) Ee e) as (σ&?&?); eauto.
     exists (Expr_type σ); simpl; split_ands; repeat typed_constructor; eauto.
   * intros m1 m2 k E e1 e2 ? (τf&HS&?&?) ?; typed_inversion HS.
-    edestruct (ectx_subst_typed_rev Γ Γf (memenv_of m1)
+    edestruct (ectx_subst_typed_rev Γ Γf ('{m1})
       (get_stack_types k) E e1) as (τrl&?&?); eauto.
     destruct (ehstep_preservation Γ Γf m1 m2 (get_stack k) (get_stack_types k)
       e1 e2 τrl) as (?&?&?); eauto using ctx_typed_stack_typed.
@@ -116,7 +115,7 @@ Proof.
     eexists; simpl; split_ands; eauto using ctx_typed_weaken,
       ectx_subst_typed, ectx_typed_weaken.
   * intros m k f' E Ωs vs ? (τf&HS&?&?) ?; typed_inversion HS.
-    edestruct (ectx_subst_typed_rev Γ Γf (memenv_of m)
+    edestruct (ectx_subst_typed_rev Γ Γf ('{m})
       (get_stack_types k) E (call f' @ #{Ωs}* vs)) as (τrl&Hcall&?); eauto.
     typed_inversion Hcall.
     split; [|eauto using funenv_typed_weaken, index_typed_unlock].
@@ -128,7 +127,7 @@ Proof.
     + repeat typed_constructor; eauto using ectx_typed_weaken,
         ctx_typed_weaken, index_typed_unlock.
   * intros m k E e ?? (τf&HS&?&?) ?; typed_inversion HS; split; auto.
-    edestruct (ectx_subst_typed_rev Γ Γf (memenv_of m)
+    edestruct (ectx_subst_typed_rev Γ Γf ('{m})
       (get_stack_types k) E e) as (τrl&?&?); eauto.
   * intros m k e Ω v (τf&HS&?&?) ?; typed_inversion HS.
     split; [|eauto using funenv_typed_weaken, index_typed_unlock].
@@ -197,7 +196,7 @@ Proof.
     eexists; simpl; split_ands; repeat typed_constructor; eauto.
     by rewrite andb_false_r.
   * intros m k f' s os vs ??? (τf&HS&?&?) ?; typed_inversion_all.
-    edestruct (funenv_lookup Γ (memenv_of m) Γf δ f')
+    edestruct (funenv_lookup Γ ('{m}) Γf δ f')
       as (s'&mτ&?&?&?&?&?&?&?); eauto.
     erewrite fmap_type_of by eauto; simplify_equality.
     edestruct (mem_alloc_val_list_valid Γ m) as (?&?&?); eauto.
@@ -230,7 +229,7 @@ Proof.
       val_typed_weaken, index_typed_valid, index_typed_representable.
     eapply stmt_typed_weaken; eauto using index_typed_free.
   * intros m k Es v s (τf&HS&?&?) ?; typed_inversion_all; split; auto.
-    edestruct (sctx_item_typed_Some_l Γ Γf (memenv_of m)
+    edestruct (sctx_item_typed_Some_l Γ Γf ('{m})
       (get_stack_types k) Es) as [??]; eauto; simplify_equality'.
     eexists; simpl; split_ands; repeat typed_constructor;
       eauto using sctx_item_subst_typed.
@@ -247,7 +246,7 @@ Proof.
       ctx_typed_weaken, index_typed_free, mem_free_valid'.
     eapply stmt_typed_weaken; eauto using index_typed_free.
   * intros m k Es l s ? (τf&HS&?&?) ?; typed_inversion HS; split; auto.
-    edestruct (sctx_item_subst_typed_rev Γ Γf (memenv_of m)
+    edestruct (sctx_item_subst_typed_rev Γ Γf ('{m})
       (get_stack_types k) Es s) as (mτ&?&?); eauto.
     eexists; simpl; split_ands; repeat typed_constructor; eauto.
   * intros m k E l s ? (τf&HS&?&?) ?; typed_inversion_all; split; auto.
@@ -255,9 +254,8 @@ Proof.
       eauto using sctx_item_subst_typed.
 Qed.
 Lemma csteps_preservation Γ Γf δ S1 S2 f :
-  ✓ Γ → Γ\ δ ⊢ₛ S1 ⇒* S2 →
-  (Γ,Γf) ⊢ S1 : f → (Γ,memenv_of (SMem S1)) ⊢ δ : Γf →
-  (Γ,Γf) ⊢ S2 : f ∧ (Γ,memenv_of (SMem S2)) ⊢ δ : Γf.
+  ✓ Γ → Γ\ δ ⊢ₛ S1 ⇒* S2 → (Γ,Γf) ⊢ S1 : f → (Γ,'{SMem S1}) ⊢ δ : Γf →
+  (Γ,Γf) ⊢ S2 : f ∧ (Γ,'{SMem S2}) ⊢ δ : Γf.
 Proof.
   induction 2 as [|S1 S2 S3]; intros; [done|].
   destruct (cstep_preservation Γ Γf δ S1 S2 f); auto.
@@ -271,7 +269,7 @@ Ltac ctx_inversion Hk :=
   | H : path_typed (V:=esctx_item _) _ _ _ _ |- _ => typed_inversion H
   end.
 Lemma cstep_progress Γ Γf δ S f :
-  ✓ Γ → (Γ,Γf) ⊢ S : f → (Γ,memenv_of (SMem S)) ⊢ δ : Γf →
+  ✓ Γ → (Γ,Γf) ⊢ S : f → (Γ,'{SMem S}) ⊢ δ : Γf →
   (**i 1.) *) red (cstep Γ δ) S ∨
   (**i 2.) *) (∃ v, final_state v S) ∨
   (**i 3.) *) undef_state S ∨
@@ -290,7 +288,7 @@ Proof.
   * destruct (is_nf_or_redex e) as [Hnf|(E&e'&?&->)].
     { destruct Hnf as [Ω v|]; typed_inversion_all.
       ctx_inversion Hk; left; try solve_cred;
-        destruct (val_true_false_dec (memenv_of m) v)
+        destruct (val_true_false_dec ('{m}) v)
         as [[[??]|[??]]|[??]]; solve_cred. }
     destruct (ehstep_exec Γ (get_stack k) e' m) as [[e'' m']|] eqn:He''.
     { apply ehstep_exec_sound in He''. left; solve_cred. }
@@ -302,7 +300,7 @@ Proof.
       * eexists; apply maybe_CCall_redex_Some; eauto.
       * edestruct ehstep_exec_weak_complete; eauto. }
     left; solve_cred.
-  * destruct (funenv_lookup Γ (memenv_of m) Γf δ f' σs σ) as (s&cmτ&?&_); auto.
+  * destruct (funenv_lookup Γ ('{m}) Γf δ f' σs σ) as (s&cmτ&?&_); auto.
     left; solve_cred.
   * ctx_inversion Hk.
     { right; left; exists v. constructor. }
@@ -311,14 +309,14 @@ Proof.
   * do 2 right; left; constructor.
 Qed.
 Lemma csteps_initial_progress Γ Γf δ m f vs S σs σ :
-  ✓ Γ → ✓{Γ} m → (Γ,memenv_of m) ⊢ δ : Γf →
-  Γf !! f = Some (σs,σ) → (Γ,memenv_of m) ⊢* vs :* σs →
+  ✓ Γ → ✓{Γ} m → (Γ,'{m}) ⊢ δ : Γf →
+  Γf !! f = Some (σs,σ) → (Γ,'{m}) ⊢* vs :* σs →
   Γ\ δ ⊢ₛ initial_state m f vs ⇒* S →
   (**i 1.) *) red (cstep Γ δ) S ∨
   (**i 2.) *) (∃ v, final_state v S) ∨
   (**i 3.) *) undef_state S.
 Proof.
-  intros. assert ((Γ,Γf) ⊢ S : f ∧ (Γ,memenv_of (SMem S)) ⊢ δ : Γf) as [??].
+  intros. assert ((Γ,Γf) ⊢ S : f ∧ (Γ,'{SMem S}) ⊢ δ : Γf) as [??].
   { eauto using csteps_preservation, initial_state_typed. }
   destruct (cstep_progress Γ Γf δ S f) as [?|[[v ?]|[?|(l&s&?&[])]]]; eauto.
   destruct S as [k φ m2]; simplify_equality'.
